some progress in HSL.fst

src/tls/HSL.fst
@@ -5,22 +5,24 @@ module HSL  // an outline of lHandshake.Log
 open Platform.Bytes
 open FStar.Heap
 open FStar.HyperHeap
+open FStar.HyperStack
 open FStar.Ghost // afer HH so as not to shadow reveal :(
-//open FStar.HyperStack
 
 ///// From Hash
 
-assume type tag: eqtype // used here both as hash tags and MAC tags 
-assume type acc
+type tag = lbytes 16 // used here both as hash tags and MAC tags 
+type acc = lbytes 16
 assume val hash: bytes -> Tot tag // computed in one step (specification)
 assume val hashA: bytes -> Tot acc   // partial computation (specification) 
 assume val extend: a0:acc -> b:bytes -> Tot (a: acc { forall (b0:bytes). a0 == hashA b0 ==> a == hashA (b0 @| b) })
 assume val finalize: a:acc -> Tot (d:tag { forall (b:bytes). a == hashA b ==> d == hash b})
+//17-01-19  I probably miss patterns
 
 ///// From Handshake.Msg
 
-assume type offer: eqtype
-type msg = | ClientHello of offer | ServerHello of offer | Finished of tag
+assume type offer: Type0
+// 17-01-19 Still confused about concrete syntax for universes + eqtypes
+noeq type msg: Type0 = | ClientHello of offer | ServerHello of offer | Finished of tag
 // simplified handshake message; for this outline we show that the client agrees with the server on the two offers after checking the Finished message
 
 assume val format: msg -> Tot bytes 
@@ -52,11 +54,10 @@ let rec tags prior incoming =
 (* STATE *)
 
 // partial flights
-type flight (prior:erased (list msg)) = ms:list msg & hs:list tag { hs = tags (reveal prior) ms }
+// type flight (prior:erased (list msg)) = ms:list msg & hs:list tag { hs = tags (reveal prior) ms }
 
 (*
 // internal state (although we may initially keep it transparent) 
-// to be wrapped in a reference 
 abstract type plainbytes i = bytes  // a shortcut: HSL merges handshake traffic at different indexes
 abstract type state = State
   transcript: erased (list Msg.t) // session transcript shared with the HS so far 
@@ -65,17 +66,18 @@ abstract type state = State
   input_msgs: flight  // partial incoming flight, hashed & parsed, with selected intermediate tags
   hash: Hash.t { hash = HashA (transcript_bytes (List.Tot.append transcript input_msgs)) } // current hash state
 *)
-type state = | State:
+noeq type state = | State:
   transcript: erased (list msg) -> // session transcript shared with the HS so far 
   input_msgs: list msg -> // partial incoming flight, hashed & parsed, with selected intermediate tags
-  input_hashes: list tag { input_hashes = tags (reveal transcript) input_msgs } -> 
-  hash: acc { hash = hashA (transcript_bytes (reveal transcript @ input_msgs)) } -> // current hash state
+  input_hashes: list tag { input_hashes == tags (reveal transcript) input_msgs } -> 
+  hash: acc { hash == hashA (transcript_bytes (reveal transcript @ input_msgs)) } -> // current hash state
   state
-type t = rref root state
+type t = r:ref state // 17-01-19 HS naming!?
 
-val transcripT: FStar.HyperHeap.t -> GTot (list msg) // the current transcript shared with the handshake
-
-let transcripT h (r:t) = (FStar.HyperHeap.sel h r).transcript
+val transcripT: h:mem -> t -> GTot (list msg) // the current transcript shared with the handshake
+let transcripT h (r:t) = 
+  let s = FStar.HyperStack.sel h r in 
+  reveal s.transcript
 
 (*
 We will also need to keep track of lengths in the input/output buffers To separate between Reading and Writing modes, a precondition for sending a message should be that both input_bytes and input_msgs are empty.(unclear who should check for emptyset, and how to react to extra bytes buffered past the input flight)
@@ -112,27 +114,28 @@ val next_fragment: t -> i:id -> ST (option fragment)
 val receive: r:t -> bytes -> ST (option (list msg * list tag))
   (requires (fun h0 -> True))
   (ensures (fun h0 o h1 -> 
-    let prior = transcripT r h0 in
+    let prior = transcripT h0 r in
     match o with 
-    | Some (ms, hs) -> transcripT r h1 = prior @ ms /\ hs = tags prior ms
-    | None -> transcripT r h1 = prior
+    | Some (ms, hs) -> transcripT h1 r == prior @ ms /\ hs = tags prior ms
+    | None -> transcripT h1 r == prior
   ))
 
 let receive r bs = 
   match parse_msg bs with // assuming bs is a potential whole message
   | None -> None
-  | Some m -> 
+  | Some m -> (
       let State transcript ms hs a = !r in
       let ms = ms @ [m]  in
       let a = extend a bs in
+      assert(a == hashA (transcript_bytes ms @| format m));
       let hs = if tagged m then (hs @ [finalize a]) else hs in
       if eoflight m then  
-        let transcript = transcript @ ms in 
-        r := State transcript [] [] a; 
-        Some (ms,hs)
-      else
+        let transcript = hide (reveal transcript @ ms) in 
+        ( r := State transcript [] [] a; 
+          Some (ms,hs) ) 
+      else (
         r := State transcript ms hs a;
-        None
+        None ))
 
 (*
 design: ghost log vs forall log?
@@ -140,21 +143,34 @@ design: how to return flights with intermediate tags?
 TODO: support multiple epochs? 
 *)
 
-
 ////// An outline of HS 
 
 assume val nego: offer -> GTot offer // the server's choice of parameters
 assume val mac_verify: h:tag -> t:tag -> 
-  Tot (b:bool { b ==> (exists offer.  h = format (ClientHello offer) @| format (ServerHello (nego offer)) ) })
+  Tot (b:bool { b ==> (exists offer.  h = hash (format (ClientHello offer) @| format (ServerHello (nego offer)))) })
 
-val process: log:t -> bytes -> c:offer -> ST (option (s:offer {s = nego c}))
-  (requires (fun h0 -> transcripT log h0 = [ClientHello c]))
-  (ensures (fun h0 r h1 -> exists tag. transcripT log h1 = [ClientHello c; ServerHello (nego c); Finished tag]))
+let inj_format c0 s0 c1 s1 : Lemma ( 
+  hash (format (ClientHello c0) @| format (ServerHello s0)) == 
+  hash (format (ClientHello c1) @| format (ServerHello s1)) ==> c0 == c1 /\ s0 == s1 ) = 
+  assume false
+
+
+val process: log:t -> bytes -> c:offer -> ST (option offer)
+  (requires (fun h0 -> transcripT h0 log == [ClientHello c]))
+  (ensures (fun h0 o h1 -> 
+    match o with 
+    | Some s -> ( s == nego c /\ (exists tag. transcripT h1 log == [ClientHello c; ServerHello s; Finished tag]))
+    | None -> transcripT h1 log == transcripT h0 log ))
 let process log (raw:bytes) client_offer = 
   match receive log raw with 
   | Some ([ServerHello server_offer; Finished tag], [hash_ch_sh]) -> 
-    if mac_verify hash_ch_sh tag then   
-    Some server_offer
+    if mac_verify hash_ch_sh tag then  (
+    assert(hash_ch_sh = hash (format (ClientHello client_offer) @| format (ServerHello (server_offer)))); 
+    assert(exists offer.  hash_ch_sh == hash (format (ClientHello offer) @| format (ServerHello (nego offer))));
+    assert(server_offer == nego client_offer);
+    assume false;
+    Some server_offer 
+    )
     else 
     None
   | _ -> None
